feat: FirstOrder.UFormula

Logic/Predicate/FirstOrder/Computability/Computability.lean
@@ -26,6 +26,16 @@ namespace UTerm
 
 instance : Inhabited (UTerm L μ) := ⟨bvar 0⟩
 
+def elim {γ : Type _} (b : ℕ → γ) (e : μ → γ) (u : {k : ℕ} → L.func k → (Fin k → γ) → γ) : UTerm L μ → γ
+  | bvar x   => b x
+  | fvar x   => e x
+  | func f v => u f (fun i => elim b e u (v i))
+
+def bind (b : ℕ → UTerm L μ₂) (e : μ₁ → UTerm L μ₂) : UTerm L μ₁ → UTerm L μ₂
+  | bvar x   => b x
+  | fvar x   => e x
+  | func f v => func f (fun i => (v i).bind b e)
+
 def rank : UTerm L μ → ℕ
   | bvar x   => x + 1
   | fvar _   => 0
@@ -47,19 +57,25 @@ def ofSubTerm : SubTerm L μ n → { t : UTerm L μ // t.rank ≤ n }
   | &x               => ⟨fvar x, by simp⟩
   | SubTerm.func f v => ⟨func f (fun i => ofSubTerm (v i)), by simp[rank]⟩
 
+lemma toSubTerm_ofSubterm {n} (t : SubTerm L μ n) : toSubTerm (ofSubTerm t).1 (ofSubTerm t).2 = t := by
+  induction t <;> simp[ofSubTerm, toSubTerm]
+  case func f v ih => { funext i; exact ih i }
+
+lemma ofSubTerm_toSubterm {n} (t : UTerm L μ) (h : t.rank ≤ n) : ofSubTerm (toSubTerm t h) = t := by
+  induction t <;> simp[ofSubTerm, toSubTerm]
+  case func f v ih =>
+    funext i
+    have h : ∀ i, (v i).rank ≤ n := by simpa[rank] using h
+    exact ih i (h i)
+
 def subtermEquivSubtype : SubTerm L μ n ≃ { t : UTerm L μ // t.rank ≤ n } where
   toFun := ofSubTerm
-  invFun := fun ⟨t, ht⟩ => t.toSubTerm ht
-  left_inv := fun t => by
-    induction t <;> simp[ofSubTerm, toSubTerm]
-    case func f v ih => { funext i; exact ih i }
-  right_inv := fun ⟨t, h⟩ => by
-    induction t <;> simp[ofSubTerm, toSubTerm]
-    case func f v ih =>
-      funext i
-      have h : ∀ i, (v i).rank ≤ n := by simpa[rank] using h
-      have : (h : (v i).rank ≤ n) → ofSubTerm (toSubTerm (v i) h) = ⟨v i, h⟩ := by simpa using ih i
-      simpa using congr_arg Subtype.val (this (h i))
+  invFun := fun t => toSubTerm t.1 t.2
+  left_inv := toSubTerm_ofSubterm
+  right_inv := by intro ⟨t, h⟩; ext; simpa using ofSubTerm_toSubterm t h
+
+open Encodable Primrec Primrec₂
+variable [Primcodable μ] [(k : ℕ) → Primcodable (L.func k)] [UniformlyPrimcodable L.func]
 
 section W
 
@@ -113,10 +129,7 @@ instance : (a : Node L μ) → Primcodable (Edge L μ a)
 instance : (a : Node L μ) → DecidableEq (Edge L μ a)
   | (Sum.inl _)                => instDecidableEqEmpty
   | (Sum.inr $ Sum.inl _)      => instDecidableEqEmpty
-  | (Sum.inr $ Sum.inr ⟨k, _⟩) => instDecidableEqFin k
-
-open Encodable Primrec Primrec₂
-variable [Primcodable μ] [(k : ℕ) → Primcodable (L.func k)] [UniformlyPrimcodable L.func]
+  | (Sum.inr $ Sum.inr ⟨k, _⟩) => instDecidableEq
 
 instance : PrimrecCard (Edge L μ) where
   card_prim :=
@@ -158,11 +171,6 @@ lemma func_primrec (k) : Primrec₂ (func : L.func k → (Fin k → UTerm L μ) 
       finArrow_map Primrec.of_equiv k
     exact (Primrec₂.comp₂ h₁ Primrec₂.left (h₂.comp₂ Primrec₂.right)).of_eq
       (fun a v => by simp[equivW, toW, Edge]; funext i; rw[Encodable.fintypeArrowEquivFinArrow'_symm_app_fin_arrow]))
-
-def elim {γ : Type _} (b : ℕ → γ) (e : μ → γ) (u : {k : ℕ} → L.func k → (Fin k → γ) → γ) : UTerm L μ → γ
-  | bvar x   => b x
-  | fvar x   => e x
-  | func f v => u f (fun i => elim b e u (v i))
 
 private def F (b : σ → ℕ → γ) (e : σ → μ → γ) (u : σ → ((k : ℕ) × L.func k) × List γ → γ) : σ → Node L μ × List γ → γ := fun z p =>
     Sum.casesOn p.1 (fun x => b z x) (fun q => Sum.casesOn q (fun x => e z x) (fun f => u z (f, p.2)))
@@ -213,13 +221,265 @@ lemma rank_primrec : Primrec (rank : UTerm L μ → ℕ) := by
     induction t <;> simp[elim, rank, *]
     { simp[List.sup_ofFn] })
 
+end W
+
 instance : Primcodable (SubTerm L μ n) :=
   letI : Primcodable { t : UTerm L μ // t.rank ≤ n } := Primcodable.subtype (nat_le.comp rank_primrec (Primrec.const n))
   Primcodable.ofEquiv { t : UTerm L μ // t.rank ≤ n } subtermEquivSubtype
+end UTerm
+
+namespace UFormula
+
+instance : Inhabited (UFormula L μ) := ⟨verum⟩
+
+def elim {γ : Type _}
+  (γVerum : γ)
+  (γFalsum : γ)
+  (γRel : {k : ℕ} → L.rel k → (Fin k → UTerm L μ) → γ)
+  (γNrel : {k : ℕ} → L.rel k → (Fin k → UTerm L μ) → γ)
+  (γAnd : γ → γ → γ)
+  (γOr : γ → γ → γ)
+  (γAll : γ → γ)
+  (γEx : γ → γ) : UFormula L μ → γ
+  | verum    => γVerum
+  | falsum   => γFalsum
+  | rel r v  => γRel r v
+  | nrel r v => γNrel r v
+  | and p q  => γAnd (p.elim γVerum γFalsum γRel γNrel γAnd γOr γAll γEx) (q.elim γVerum γFalsum γRel γNrel γAnd γOr γAll γEx)
+  | or p q   => γOr (p.elim γVerum γFalsum γRel γNrel γAnd γOr γAll γEx) (q.elim γVerum γFalsum γRel γNrel γAnd γOr γAll γEx)
+  | all p    => γAll (p.elim γVerum γFalsum γRel γNrel γAnd γOr γAll γEx)
+  | ex p     => γEx (p.elim γVerum γFalsum γRel γNrel γAnd γOr γAll γEx)
+
+def rank : UFormula L μ → ℕ
+  | verum    => 0
+  | falsum   => 0
+  | rel _ v  => Finset.sup Finset.univ (fun i => (v i).rank)
+  | nrel _ v => Finset.sup Finset.univ (fun i => (v i).rank)
+  | and p q  => max p.rank q.rank
+  | or p q   => max p.rank q.rank
+  | all p    => p.rank.pred
+  | ex p     => p.rank.pred
+
+@[simp] lemma rank_verum : rank (verum : UFormula L μ) = 0 := rfl
+
+@[simp] lemma rank_falsum : rank (falsum : UFormula L μ) = 0 := rfl
+
+@[simp] lemma rank_rel {k} (r : L.rel k) (v : Fin k → UTerm L μ) : rank (rel r v) = Finset.sup Finset.univ (fun i => (v i).rank) := rfl
+
+@[simp] lemma rank_nrel {k} (r : L.rel k) (v : Fin k → UTerm L μ) : rank (nrel r v) = Finset.sup Finset.univ (fun i => (v i).rank) := rfl
+
+@[simp] lemma rank_and (p q : UFormula L μ) : (and p q).rank = max p.rank q.rank := rfl
+
+@[simp] lemma rank_or (p q : UFormula L μ) : (or p q).rank = max p.rank q.rank := rfl
+
+@[simp] lemma rank_all (p : UFormula L μ) : (all p).rank = p.rank.pred := rfl
+
+@[simp] lemma rank_ex (p : UFormula L μ) : (ex p).rank = p.rank.pred := rfl
+
+@[simp] lemma subtype_val_le (p : { p : UFormula L μ // p.rank ≤ n }) : p.val.rank ≤ n := p.property
+
+def toSubFormula : {n : ℕ} → (p : UFormula L μ) → p.rank ≤ n → SubFormula L μ n
+  | _, verum,    _ => ⊤
+  | _, falsum,   _ => ⊥
+  | _, rel r v,  h => SubFormula.rel r (fun i => (v i).toSubTerm (by simp at h; exact h i))
+  | _, nrel r v, h => SubFormula.nrel r (fun i => (v i).toSubTerm (by simp at h; exact h i))
+  | _, and p q,  h => p.toSubFormula (by simp at h; exact h.1) ⋏ q.toSubFormula (by simp at h; exact h.2)
+  | _, or p q,   h => p.toSubFormula (by simp at h; exact h.1) ⋎ q.toSubFormula (by simp at h; exact h.2)
+  | _, all p,    h => ∀' p.toSubFormula (Nat.le_add_of_sub_le h)
+  | _, ex p,     h => ∃' p.toSubFormula (Nat.le_add_of_sub_le h)
+
+def ofSubFormula : {n : ℕ} → SubFormula L μ n → { p : UFormula L μ // p.rank ≤ n }
+  | _, ⊤                   => ⟨verum, by simp⟩
+  | _, ⊥                   => ⟨falsum, by simp⟩
+  | _, SubFormula.rel r v  => ⟨rel r (fun i => (UTerm.ofSubTerm $ v i)), by simp⟩
+  | _, SubFormula.nrel r v => ⟨nrel r (fun i => (UTerm.ofSubTerm $ v i)), by simp⟩
+  | _, p ⋏ q               => ⟨and (ofSubFormula p) (ofSubFormula q), by simp⟩
+  | _, p ⋎ q               => ⟨or (ofSubFormula p) (ofSubFormula q), by simp⟩
+  | _, ∀' p                => ⟨all (ofSubFormula p), by simpa using Iff.mpr Nat.pred_le_iff (ofSubFormula p).property⟩
+  | _, ∃' p                => ⟨ex (ofSubFormula p), by simpa using Iff.mpr Nat.pred_le_iff (ofSubFormula p).property⟩
+
+lemma toSubFormula_ofSubFormula : ∀ {n : ℕ} (p : SubFormula L μ n), toSubFormula (ofSubFormula p).1 (ofSubFormula p).2 = p
+  | _, ⊤                   => rfl
+  | _, ⊥                   => rfl
+  | _, SubFormula.rel r v  => by simp[ofSubFormula, toSubFormula, UTerm.toSubTerm_ofSubterm]
+  | _, SubFormula.nrel r v => by simp[ofSubFormula, toSubFormula, UTerm.toSubTerm_ofSubterm]
+  | _, p ⋏ q               => by simp[ofSubFormula, toSubFormula]; exact ⟨toSubFormula_ofSubFormula p, toSubFormula_ofSubFormula q⟩
+  | _, p ⋎ q               => by simp[ofSubFormula, toSubFormula]; exact ⟨toSubFormula_ofSubFormula p, toSubFormula_ofSubFormula q⟩
+  | _, ∀' p                => by simp[ofSubFormula, toSubFormula]; exact toSubFormula_ofSubFormula p
+  | _, ∃' p                => by simp[ofSubFormula, toSubFormula]; exact toSubFormula_ofSubFormula p
+
+lemma ofSubFormula_toSubFormula : ∀ {n : ℕ} (p : UFormula L μ) (h : p.rank ≤ n), ofSubFormula (toSubFormula p h) = p
+  | _, verum,    h => rfl
+  | _, falsum,   h => rfl
+  | _, rel r v,  h => by simp[ofSubFormula, toSubFormula, UTerm.ofSubTerm_toSubterm]
+  | _, nrel r v, h => by simp[ofSubFormula, toSubFormula, UTerm.ofSubTerm_toSubterm]
+  | _, and p q,  h => by
+    simp[ofSubFormula, toSubFormula]
+    exact ⟨ofSubFormula_toSubFormula p (by simp at h; exact h.1), ofSubFormula_toSubFormula q (by simp at h; exact h.2)⟩
+  | _, or p q,   h => by
+    simp[ofSubFormula, toSubFormula]
+    exact ⟨ofSubFormula_toSubFormula p (by simp at h; exact h.1), ofSubFormula_toSubFormula q (by simp at h; exact h.2)⟩
+  | _, all p,    h => by
+    simp[ofSubFormula, toSubFormula]
+    exact ofSubFormula_toSubFormula p (by {simp at h; exact Nat.le_add_of_sub_le h })
+  | _, ex p,     h => by
+    simp[ofSubFormula, toSubFormula]
+    exact ofSubFormula_toSubFormula p (by {simp at h; exact Nat.le_add_of_sub_le h })
+
+def subformulaEquivSubtype : SubFormula L μ n ≃ { p : UFormula L μ // p.rank ≤ n } where
+  toFun := ofSubFormula
+  invFun := fun p => p.1.toSubFormula p.2
+  left_inv := toSubFormula_ofSubFormula
+  right_inv := fun ⟨p, h⟩ => by ext; simpa using ofSubFormula_toSubFormula p h
+
+open Encodable Primrec Primrec₂
+variable [(k : ℕ) → Primcodable (L.func k)] [(k : ℕ) → Primcodable (L.rel k)]
+  [UniformlyPrimcodable L.func] [UniformlyPrimcodable L.rel] [Primcodable μ]
+
+section W
+
+abbrev Node (L : Language.{u}) (μ : Type v) :=
+  Bool × (((k : ℕ) × L.rel k × (Fin k → UTerm L μ)) ⊕ Unit ⊕ Unit ⊕ Unit)
+-- sign × (atomic formula ⊕ ⊤/⊥ ⊕ ⋏/⋎ ⊕ ∀/∃)
+
+instance : Primcodable (Node L μ) := Primcodable.prod
+
+@[reducible] def Edge (L : Language.{u}) (μ : Type v) : Node L μ → Type
+  | (_, Sum.inl ⟨_, _, _⟩)              => Empty
+  | (_, Sum.inr $ Sum.inl ())           => Empty
+  | (_, Sum.inr $ Sum.inr $ Sum.inl ()) => Bool
+  | (_, Sum.inr $ Sum.inr $ Sum.inr ()) => Unit
+
+def toW : UFormula L μ → WType (Edge L μ)
+  | rel r v  => ⟨(true,  Sum.inl ⟨_, r, v⟩), Empty.elim⟩
+  | nrel r v => ⟨(false, Sum.inl ⟨_, r, v⟩), Empty.elim⟩
+  | verum    => ⟨(true,  Sum.inr $ Sum.inl ()), Empty.elim⟩
+  | falsum   => ⟨(false, Sum.inr $ Sum.inl ()), Empty.elim⟩
+  | and p q  => ⟨(true,  Sum.inr $ Sum.inr $ Sum.inl ()), Bool.rec p.toW q.toW⟩
+  | or p q   => ⟨(false, Sum.inr $ Sum.inr $ Sum.inl ()), Bool.rec p.toW q.toW⟩
+  | all p    => ⟨(true,  Sum.inr $ Sum.inr $ Sum.inr ()), fun _ => p.toW⟩
+  | ex p     => ⟨(false, Sum.inr $ Sum.inr $ Sum.inr ()), fun _ => p.toW⟩
+
+def ofW : WType (Edge L μ) → UFormula L μ
+  | ⟨(true,  Sum.inl ⟨_, r, v⟩), _⟩              => rel r v
+  | ⟨(false, Sum.inl ⟨_, r, v⟩), _⟩              => nrel r v
+  | ⟨(true,  Sum.inr $ Sum.inl ()), _⟩           => verum
+  | ⟨(false, Sum.inr $ Sum.inl ()), _⟩           => falsum
+  | ⟨(true,  Sum.inr $ Sum.inr $ Sum.inl ()), p⟩ => and (ofW $ p false) (ofW $ p true)
+  | ⟨(false, Sum.inr $ Sum.inr $ Sum.inl ()), p⟩ => or (ofW $ p false) (ofW $ p true)
+  | ⟨(true,  Sum.inr $ Sum.inr $ Sum.inr ()), p⟩ => all (ofW $ p ())
+  | ⟨(false, Sum.inr $ Sum.inr $ Sum.inr ()), p⟩ => ex (ofW $ p ())
+
+lemma toW_ofW : ∀ (w : WType (Edge L μ)), toW (ofW w) = w
+  | ⟨(true,  Sum.inl ⟨_, r, v⟩), _⟩              => by simp[ofW, toW]
+  | ⟨(false, Sum.inl ⟨_, r, v⟩), _⟩              => by simp[ofW, toW]
+  | ⟨(true,  Sum.inr $ Sum.inl ()), _⟩           => by simp[ofW, toW]
+  | ⟨(false, Sum.inr $ Sum.inl ()), _⟩           => by simp[ofW, toW]
+  | ⟨(true,  Sum.inr $ Sum.inr $ Sum.inl ()), w⟩ => by
+    simp[ofW, toW, toW_ofW (w false), toW_ofW (w true)]
+    ext b; cases b <;> simp
+  | ⟨(false, Sum.inr $ Sum.inr $ Sum.inl ()), w⟩ => by
+    simp[ofW, toW, toW_ofW (w false), toW_ofW (w true)]
+    ext b; cases b <;> simp
+  | ⟨(true,  Sum.inr $ Sum.inr $ Sum.inr ()), w⟩ => by simp[ofW, toW, toW_ofW (w ())]
+  | ⟨(false, Sum.inr $ Sum.inr $ Sum.inr ()), w⟩ => by simp[ofW, toW, toW_ofW (w ())]
+
+def equivW (L) (μ) : UFormula L μ ≃ WType (Edge L μ) where
+  toFun := toW
+  invFun := ofW
+  left_inv := fun p => by induction p <;> simp[toW, ofW, *]
+  right_inv := toW_ofW
+
+@[simp] lemma equivW_symm_true_inr_inr_inl (v : Bool → WType (Edge L μ)) :
+    (equivW L μ).symm ⟨(true, Sum.inr $ Sum.inr $ Sum.inl ()), v⟩ = and ((equivW L μ).symm $ v false) ((equivW L μ).symm $ v true) := rfl
+
+@[simp] lemma equivW_symm_false_inr_inr_inl (v : Bool → WType (Edge L μ)) :
+    (equivW L μ).symm ⟨(false, Sum.inr $ Sum.inr $ Sum.inl ()), v⟩ = or ((equivW L μ).symm $ v false) ((equivW L μ).symm $ v true) := rfl
+
+@[simp] lemma equivW_symm_true_inr_inr_inr (v : Unit → WType (Edge L μ)) :
+    (equivW L μ).symm ⟨(true, Sum.inr $ Sum.inr $ Sum.inr ()), v⟩ = all ((equivW L μ).symm $ v ()) := rfl
+
+@[simp] lemma equivW_symm_false_inr_inr_inr (v : Unit → WType (Edge L μ)) :
+    (equivW L μ).symm ⟨(false, Sum.inr $ Sum.inr $ Sum.inr ()), v⟩ = ex ((equivW L μ).symm $ v ()) := rfl
+
+instance : (a : Node L μ) → Fintype (Edge L μ a)
+  | (_, Sum.inl ⟨_, _, _⟩)              => Fintype.ofIsEmpty
+  | (_, Sum.inr $ Sum.inl ())           => Fintype.ofIsEmpty
+  | (_, Sum.inr $ Sum.inr $ Sum.inl ()) => Bool.fintype
+  | (_, Sum.inr $ Sum.inr $ Sum.inr ()) => Unique.fintype
+
+instance : (a : Node L μ) → Primcodable (Edge L μ a)
+  | (_, Sum.inl ⟨_, _, _⟩)              => Primcodable.empty
+  | (_, Sum.inr $ Sum.inl ())           => Primcodable.empty
+  | (_, Sum.inr $ Sum.inr $ Sum.inl ()) => Primcodable.bool
+  | (_, Sum.inr $ Sum.inr $ Sum.inr ()) => Primcodable.unit
+
+instance : (a : Node L μ) → DecidableEq (Edge L μ a)
+  | (_, Sum.inl ⟨_, _, _⟩)              => instDecidableEqEmpty
+  | (_, Sum.inr $ Sum.inl ())           => instDecidableEqEmpty
+  | (_, Sum.inr $ Sum.inr $ Sum.inl ()) => instDecidableEq
+  | (_, Sum.inr $ Sum.inr $ Sum.inr ()) => instDecidableEq
+
+instance : PrimrecCard (Edge L μ) where
+  card_prim :=
+    have : Primrec
+      ( fun a => Sum.casesOn a.2 (fun _ => 0)
+        $ fun c => Sum.casesOn c (fun _ => 0)
+        $ fun c => Sum.casesOn c (fun _ => 2)
+        $ fun _ => 1 : Node L μ → ℕ) :=
+      by apply sum_casesOn snd (const 0)
+          (by apply sum_casesOn snd (const 0)
+                (by apply sum_casesOn snd (const 2) (const 1)))
+    this.of_eq (fun (_, c) => by
+      rcases c with (_ | c) <;> simp[Edge]
+      rcases c with (_ | c) <;> simp[Edge]
+      rcases c <;> simp[Edge])
+
+instance primcodable : Primcodable (UFormula L μ) := Primcodable.ofEquiv (WType (Edge L μ)) (equivW L μ)
+
+/-
+lemma relL_primrec :
+  Primrec₂ (fun (f : (k : ℕ) × L.rel k) (l : List (UTerm L μ)) =>
+    if h : l.length = f.1
+      then some (rel f.2 (fun i => l.get (i.cast h.symm)))
+      else none) := by
+  let i : (k : ℕ) × L.rel k × (Fin k → UTerm L μ) → Node L μ := fun t => (true, Sum.inl ⟨t.1, t.2.1, t.2.2⟩)
+  have : Primrec i := sorry
+  have : Primrec (fun t => WType.mk (i t) Empty.elim) :=
+    w_mk₀ (β := Edge L μ) i (by intros; exact instIsEmptyEmpty) this
+-/
+
+lemma and_primrec : Primrec₂ (and : UFormula L μ → UFormula L μ → UFormula L μ) := by
+  have := w_mk₂ (β := Edge L μ) (fun (_ : Unit) => (true, Sum.inr $ Sum.inr $ Sum.inl ())) (by rintro ⟨⟩; simp[Edge]) (const _)
+  have := (Primrec.of_equiv_symm (e := equivW L μ)).comp₂
+    ((this.comp₂ (Primrec₂.const ()) Primrec.id.to₂).comp₂
+      ((Primrec.of_equiv (e := equivW L μ)).comp₂ Primrec₂.left)
+      ((Primrec.of_equiv (e := equivW L μ)).comp₂ Primrec₂.right))
+  exact this.of_eq (fun p q => by simp; rw[fintypeEquivFin_false, fintypeEquivFin_true]; simp)
+
+lemma or_primrec : Primrec₂ (or : UFormula L μ → UFormula L μ → UFormula L μ) := by
+  have := w_mk₂ (β := Edge L μ) (fun (_ : Unit) => (false, Sum.inr $ Sum.inr $ Sum.inl ())) (by rintro ⟨⟩; simp[Edge]) (const _)
+  have := (Primrec.of_equiv_symm (e := equivW L μ)).comp₂
+    ((this.comp₂ (Primrec₂.const ()) Primrec.id.to₂).comp₂
+      ((Primrec.of_equiv (e := equivW L μ)).comp₂ Primrec₂.left)
+      ((Primrec.of_equiv (e := equivW L μ)).comp₂ Primrec₂.right))
+  exact this.of_eq (fun p q => by simp; rw[fintypeEquivFin_false, fintypeEquivFin_true]; simp)
+
+lemma all_primrec : Primrec (all : UFormula L μ → UFormula L μ) := by
+  have := w_mk₁ (β := Edge L μ) (fun (_ : Unit) => (true, Sum.inr $ Sum.inr $ Sum.inr ())) (by rintro ⟨⟩; simp[Edge]) (const _)
+  have := (Primrec.of_equiv_symm (e := equivW L μ)).comp
+    ((this.comp (Primrec.const ()) Primrec.id).comp (Primrec.of_equiv (e := equivW L μ)))
+  exact this.of_eq (fun p => by simp)
+
+lemma ex_primrec : Primrec (ex : UFormula L μ → UFormula L μ) := by
+  have := w_mk₁ (β := Edge L μ) (fun (_ : Unit) => (false, Sum.inr $ Sum.inr $ Sum.inr ())) (by rintro ⟨⟩; simp[Edge]) (const _)
+  have := (Primrec.of_equiv_symm (e := equivW L μ)).comp
+    ((this.comp (Primrec.const ()) Primrec.id).comp (Primrec.of_equiv (e := equivW L μ)))
+  exact this.of_eq (fun p => by simp)
 
 end W
 
-end UTerm
+end UFormula
 
 end FirstOrder
 
